src/ecUnify.ml
@@ -114,7 +114,7 @@ module UnifyGen(X : UnifyExtra) = struct
       (uf, tuni uid)
 
   (* ------------------------------------------------------------------ *)
-  let rec unify_core (env : EcEnv.env) (tvtc : X.state Mid.t) (uf : UF.t) pb =
+  let unify_core (env : EcEnv.env) (tvtc : X.state Mid.t) (uf : UF.t) pb =
     let failure () = raise (UnificationFailure pb) in
 
     let uf = ref uf in
@@ -297,6 +297,14 @@ module TypeClass = struct
       let tvinst =
         List.map
           (fun (tv, tcs) ->
+             List.map (fun tc -> (([], tvar tv), tc)) tcs)
+          (Mid.bindings tvtc)
+      in List.flatten tvinst @ instances in
+
+(*
+      let tvinst =
+        List.map
+          (fun (tv, tcs) ->
              let rec parent_instances_of_tc acc tc =
                let acc    = (([], tvar tv), tc) :: acc in
                let tcdecl = EcEnv.TypeClass.by_path tc.tc_name env in
@@ -316,19 +324,46 @@ module TypeClass = struct
           (Mid.bindings tvtc)
 
       in List.flatten (List.flatten tvinst) @ instances in
+*)
 
     let exception Bailout in
 
+    let rec find_tc_in_parent acc tginst =
+      if EcPath.p_equal tc.tc_name tginst.tc_name then
+        Some (tginst.tc_args, List.rev acc)
+      else
+        let tcdecl = EcEnv.TypeClass.by_path tginst.tc_name env in
+        tcdecl.tc_prt |> obind (fun prt ->
+          let acc = (tcdecl.tc_tparams, tginst.tc_args) :: acc in
+          find_tc_in_parent acc prt) in
+
     let for1 ((tgparams, tgty), tginst) =
-      if not (EcPath.p_equal tc.tc_name tginst.tc_name) then
-        raise Bailout;
+      let tgi_args, tgparams_prt  =
+        oget ~exn:Bailout (find_tc_in_parent [] tginst) in
 
       let uf, tvinfo =
         List.fold_left_map
           (fun uf (tv, tcs) ->
             let uf, tvty = UnifyCore.fresh uf in uf, (tv, (tvty, tcs)))
           UnifyCore.UF.initial tgparams in
-      let uf, subst = ref uf, Mid.of_list (List.map (snd_map fst) tvinfo) in
+
+      let subst =
+        Mid.of_list (List.map (snd_map fst) tvinfo) in
+
+      let subst =
+        let tcsubst =
+          List.fold_left
+            (fun subst (tparams, args) ->
+               let args  = List.map (Tvar.subst subst) args in
+               let subst = List.combine (List.fst tparams) args in
+               Mid.of_list subst)
+            subst tgparams_prt in
+
+        Mid.fold
+          (fun x ty subst -> Mid.add x ty subst)
+          tcsubst subst in
+
+      let uf, tgi_args = ref uf, List.map (Tvar.subst subst) tgi_args in
 
       List.iter2
         (fun pty tgty ->
@@ -337,7 +372,7 @@ module TypeClass = struct
              uf := UnifyCore.unify_core env Mid.empty !uf (`TyUni (pty, tgty))
            with UnifyCore.UnificationFailure _ ->
              raise Bailout)
-        tc.tc_args tginst.tc_args;
+        tc.tc_args tgi_args;
 
       let tgty = Tvar.subst subst tgty in
 
